

$$T_{ON} = \frac{1}{K_{ON} C_{A0} (\alpha - 1)} \ln \left[\frac{\alpha - x}{\alpha(1-x)} \right]$$

Now conversion = Y

$$r = K_{OFF} C_A C_B$$

$$C_{new} = C_{A0}(1-x)$$

$$\left(\frac{dC_A}{dt} \right) = K_{OFF} C_{A_{new}}(1-Y) (C_{B_{new}} - C_{A0}x - C_{A_{new}}Y)$$

$$\frac{dY}{dt} = K_{OFF} C_{A0}(1-x)(1-y) \left(\frac{C_{B0} - C_{A0}x}{C_{A0}(1-x)} - y \right)$$

$$\frac{dy}{(1-y) \left(\frac{C_{B0} - C_{A0}x}{C_{A0}(1-x)} - y \right)} = \int_0^t dt (K_{OFF} C_{A0}(1-x))$$

Integration both sides

& simplifying for T_{OFF}

$$T_{OFF} = \frac{1}{(\alpha - 1)(C_{A0}(1-x))} \ln \left(\frac{(\alpha - Y)(1-x)}{(\alpha - x)(1-y)} \right)$$

$$T_{total} = T_{ON} + T_{OFF} + T_{ON} + T_{OFF}$$

→ using this result we can

generalise for ~~other~~ next T_{ON} & T_{OFF}